identity pass almost done -- just need to prove preservation for chkc

cfrontend/ChkCgenproof.v
@@ -16,7 +16,7 @@ Require Import FunInd.
 Require Import Coqlib Maps Errors Integers.
 Require Import AST Linking.
 Require Import Values Memory Events Globalenvs Smallstep.
-Require Import Ctypes Cop ChkCsyntax Csyntax Csem Cstrategy Clight.
+Require Import Ctypes Cop ChkCsyntax Csyntax ChkCsem Csem ChkCstrategy Cstrategy.
 Require Import ChkCgen ChkCgenspec.
 
 (** ** Relational specification of the translation. *)
@@ -33,6 +33,93 @@ Proof.
   eapply match_transform_partial_program_contextual. eexact EQ.
   intros. apply transl_fundef_spec; auto.
 Qed.
+
+Section PRESERVATION.
+
+  Variable prog: ChkCsyntax.program.
+  Variable tprog: Csyntax.program.
+  Hypothesis TRANSL: match_prog prog tprog.
+
+  Let ge := ChkCsem.globalenv prog.
+  Let tge := Csem.globalenv tprog.
+
+  Lemma senv_preserved:
+    Senv.equiv ge tge.
+  Proof.
+    Admitted.
+(* (Genv.senv_match (proj1 TRANSL)). *)
+
+
+  (** Anti-stuttering measure *)
+
+(** There are some stuttering steps in the translation:
+- The execution of [Sdo a] where [a] is side-effect free,
+  which is three transitions in the source:
+<<
+    Sdo a, k  --->  a, Kdo k ---> rval v, Kdo k ---> Sskip, k
+>>
+  but the translation, which is [Sskip], makes no transitions.
+- The reduction [Ecomma (Eval v) r2 --> r2].
+- The reduction [Eparen (Eval v) --> Eval v] in a [For_effects] context.
+
+The following measure decreases for these stuttering steps. *)
+
+Fixpoint esize (a: ChkCsyntax.expr) : nat :=
+  match a with
+  | ChkCsyntax.Eloc _ _ _ => 1%nat
+  | ChkCsyntax.Evar _ _ => 1%nat
+  | ChkCsyntax.Ederef r1 _ => S(esize r1)
+  | ChkCsyntax.Efield l1 _ _ => S(esize l1)
+  | ChkCsyntax.Eval _ _ => O
+  | ChkCsyntax.Evalof l1 _ => S(esize l1)
+  | ChkCsyntax.Eaddrof l1 _ => S(esize l1)
+  | ChkCsyntax.Eunop _ r1 _ => S(esize r1)
+  | ChkCsyntax.Ebinop _ r1 r2 _ => S(esize r1 + esize r2)%nat
+  | ChkCsyntax.Ecast r1 _ => S(esize r1)
+  | ChkCsyntax.Eseqand r1 _ _ => S(esize r1)
+  | ChkCsyntax.Eseqor r1 _ _ => S(esize r1)
+  | ChkCsyntax.Econdition r1 _ _ _ => S(esize r1)
+  | ChkCsyntax.Esizeof _ _ => 1%nat
+  | ChkCsyntax.Ealignof _ _ => 1%nat
+  | ChkCsyntax.Eassign l1 r2 _ => S(esize l1 + esize r2)%nat
+  | ChkCsyntax.Eassignop _ l1 r2 _ _ => S(esize l1 + esize r2)%nat
+  | ChkCsyntax.Epostincr _ l1 _ => S(esize l1)
+  | ChkCsyntax.Ecomma r1 r2 _ => S(esize r1 + esize r2)%nat
+  | ChkCsyntax.Ecall r1 rl2 _ => S(esize r1 + esizelist rl2)%nat
+  | ChkCsyntax.Ebuiltin ef _ rl _ => S(esizelist rl)%nat
+  | ChkCsyntax.Eparen r1 _ _ => S(esize r1)
+  end
+
+with esizelist (el: ChkCsyntax.exprlist) : nat :=
+  match el with
+  | ChkCsyntax.Enil => O
+  | ChkCsyntax.Econs r1 rl2 => (esize r1 + esizelist rl2)%nat
+  end.
+
+Definition measure (st: ChkCsem.state) : nat :=
+  match st with
+  | ChkCsem.ExprState _ r _ _ _ => (esize r + 1)%nat
+  | ChkCsem.State _ ChkCsyntax.Sskip _ _ _ => 0%nat
+  | ChkCsem.State _ (ChkCsyntax.Sdo r) _ _ _ => (esize r + 2)%nat
+  | ChkCsem.State _ (ChkCsyntax.Sifthenelse r _ _) _ _ _ => (esize r + 2)%nat
+  | _ => 0%nat
+  end.
+
+Theorem transl_program_correct:
+  forward_simulation (ChkCstrategy.semantics prog) (Cstrategy.semantics tprog).
+Proof.
+Admitted.
+(*
+  eapply forward_simulation_star_wf with (order := ltof _ measure).
+  eapply senv_preserved.
+  eexact transl_initial_states.
+  eexact transl_final_states.
+  apply well_founded_ltof.
+  exact simulation.
+Qed.
+*)
+
+End PRESERVATION.
 
 Instance TransfChkCGenLink : TransfLink match_prog.
 Proof.
