Makefile
@@ -98,7 +98,7 @@ BACKEND=\
 
 # C front-end modules (in cfrontend/)
 
-CFRONTEND=Ctypes.v Cop.v ChkCsyntax.v Csyntax.v Csem.v Ctyping.v Cstrategy.v Cexec.v \
+CFRONTEND=Ctypes.v Cop.v ChkCsyntax.v Csyntax.v ChkCsem.v Csem.v Ctyping.v ChkCstrategy.v Cstrategy.v Cexec.v \
   Initializers.v Initializersproof.v \
   ChkCgen.v ChkCgenspec.v ChkCgenproof.v SimplExpr.v SimplExprspec.v SimplExprproof.v \
   Clight.v ClightBigstep.v SimplLocals.v SimplLocalsproof.v \
